{
 "cells": [
  {
   "cell_type": "markdown",
   "metadata": {},
   "source": [
    "# (a)"
   ]
  },
  {
   "cell_type": "markdown",
   "metadata": {},
   "source": [
    "Use $(k)$ instead of $(i)$ for indexing data point to avoid confusion later, and use $i$ and $j$ to index the dimensions of $x$. Suppose the $x^{(k)}$ is a $n$-dimension vector.\n",
    "\n",
    "\\begin{align*}\n",
    "J(\\theta) &= \\frac{1}{m} \\sum_{k=1}^{m} \\mathrm{log}(1 + e ^{-y^{(k)} \\theta^T x^{(i)})} \\\\\n",
    "               &= - \\frac{1}{m} \\sum_{k=1}^{m} \\mathrm{log}(g(z))\n",
    "\\end{align*}\n",
    "\n",
    "where $g(z) = \\frac{1}{1 + e^{-z}}$ and $z = y^{(i)} \\theta^T x^{(i)}$"
   ]
  },
  {
   "cell_type": "markdown",
   "metadata": {},
   "source": [
    "Note that\n",
    "\\begin{align*}\n",
    "\\frac{\\partial g}{\\partial z} =\\frac{\\partial \\frac{1}{1 + e^{-z}}}{\\partial z}  \n",
    "                              =\\frac{0 - 1 \\times \\frac{\\partial (1 + e^{-z})}{\\partial z}}{(1 + e^{-z})^2} \n",
    "                              =\\frac{e^{-z}}{(1 + e^{-z})^2} \n",
    "                              =\\frac{1}{1 + e^{-z}} \\cdot \\frac{e^{-z}}{1 + e^{-z}}\n",
    "                              =g(1 - g)\n",
    "\\end{align*}"
   ]
  },
  {
   "cell_type": "markdown",
   "metadata": {},
   "source": [
    "and similarly (unnecessary for this problem, just put here for reference),\n",
    "\n",
    "\\begin{align*}\n",
    "\\frac{\\partial (1 - g)}{\\partial z} \n",
    "= \\frac{\\partial \\frac{e^{-z}}{1 + e^{-z}}}{\\partial z}\n",
    "= - \\frac{\\partial g}{\\partial z} = g(g - 1)\n",
    "\\end{align*}"
   ]
  },
  {
   "cell_type": "markdown",
   "metadata": {},
   "source": [
    "So\n",
    "\n",
    "\\begin{align*}\n",
    "\\frac{\\partial J}{\\partial \\theta_i} \n",
    " &= -\\frac{1}{m} \\sum_{k=1}^{m} \\frac{1}{g(z)} \\frac{\\partial g(z)}{\\partial z} \\frac{\\partial z(\\theta_i)}{\\partial \\theta_i}  \\\\\n",
    " &= -\\frac{1}{m} \\sum_{k=1}^{m} \\frac{1}{g(z)} g(z) (1 - g(z)) \\frac{\\partial z}{\\partial \\theta_i}  \\\\\n",
    " &= -\\frac{1}{m} \\sum_{k=1}^{m} (1 - g(z)) \\frac{\\partial z}{\\partial \\theta_i}  \\\\\n",
    " &= -\\frac{1}{m} \\sum_{k=1}^{m} (1 - g(z)) y^{(k)} x_i^{(k)}  \\\\\n",
    " &= \\frac{1}{m} \\sum_{k=1}^{m} (g(z) - 1) y^{(k)} x_i^{(k)}  \\\\\n",
    "\\end{align*}\n"
   ]
  },
  {
   "cell_type": "markdown",
   "metadata": {},
   "source": [
    "Then,\n",
    "\n",
    "\\begin{align*}\n",
    "H_{ij} = \\frac{\\partial J}{\\partial \\theta_i \\theta_j} \n",
    "&= \\frac{1}{m} \\sum_{k=1}^{m} \\frac{\\partial (g(z)  - 1)}{\\partial \\theta_j} y^{(k)} x_i^{(k)} \\\\\n",
    "&= \\frac{1}{m} \\sum_{k=1}^{m} \\frac {\\partial g(z)}{\\partial \\theta_j} y^{(k)} x_i^{(k)} \\\\\n",
    "&= \\frac{1}{m} \\sum_{k=1}^{m} g(z)(1 - g(z)) \\frac{\\partial z}{\\partial \\theta_j} y^{(k)} x_i^{(k)} \\\\\n",
    "&= \\frac{1}{m} \\sum_{k=1}^{m} g(z)(1 - g(z)) y^{(k)} x_j^{(k)} y^{(k)} x_i^{(k)} \\\\\n",
    "&= \\frac{1}{m} \\sum_{k=1}^{m} g(z)(1 - g(z)) x_i^{(k)} x_j^{(k)} \\\\\n",
    "\\end{align*}"
   ]
  },
  {
   "cell_type": "markdown",
   "metadata": {},
   "source": [
    "Lastly,\n",
    "\\begin{align*}\n",
    "z^THz &= \\sum_{i=1}^{m} \\sum_{j=1}^{m} z_i H_{ij} z_j \\\\\n",
    "           &= \\sum_{i=1}^{n} \\sum_{j=1}^{n} [z_i \\frac{1}{m} \\sum_{k=1}^{m} g(z)(1 - g(z)) x_i^{(k)} x_j^{(k)}] z_j \\\\\n",
    "           &= \\frac{1}{m} \\sum_{k=1}^{m} g(z)(1 - g(z)) \\sum_{i=1}^{n} \\sum_{j=1}^{n} z_i x_i^{(k)} x_j^{(k)} z_j\n",
    "\\end{align*}"
   ]
  },
  {
   "cell_type": "markdown",
   "metadata": {},
   "source": [
    "Given that $1 > g(z) > 0$ and $\\sum_{i=1}^{n} \\sum_{j=1}^{n} z_i x_i^{(k)} x_j^{(k)} z_j = ((x^{(k)})^T z)^2 \\ge 0$, \n",
    "\n",
    "$z^T H z \\ge 0$, so $H$ is PSD, i.e. $H \\succeq 0$. \n",
    "\n",
    "Hence, $J$ is convex and it has no local minima."
   ]
  },
  {
   "cell_type": "code",
   "execution_count": null,
   "metadata": {
    "collapsed": true
   },
   "outputs": [],
   "source": []
  }
 ],
 "metadata": {
  "anaconda-cloud": {},
  "kernelspec": {
   "display_name": "Python 3",
   "language": "python",
   "name": "python3"
  },
  "language_info": {
   "codemirror_mode": {
    "name": "ipython",
    "version": 3
   },
   "file_extension": ".py",
   "mimetype": "text/x-python",
   "name": "python",
   "nbconvert_exporter": "python",
   "pygments_lexer": "ipython3",
   "version": "3.5.1"
  }
 },
 "nbformat": 4,
 "nbformat_minor": 0
}
